Lifted stypes over OFEs
Squashed commit of the following:

commit b404feb30cecf7678c0ad6007171a13361483086
Author: Jonas Kastberg Hinrichsen <jkas@itu.dk>
Date:   Wed Apr 17 17:36:21 2019 +0200

    Bumped try_recv and recv to ofe st's

commit 4aa2399d02de67feacdcba9d0929cd7e20a1f7da
Author: Jonas Kastberg Hinrichsen <jkas@itu.dk>
Date:   Wed Apr 17 15:19:14 2019 +0200

    Finalised send proof

commit ae9857fcf8a88e917b6ccb219ac6e27a1afe46e2
Author: Robbert Krebbers <mail@robbertkrebbers.nl>
Date:   Wed Apr 17 14:58:34 2019 +0200

    Tweak.

commit 4d86571d9d51992d6ee83fdfbbfbec24ce8fdbc8
Author: Robbert Krebbers <mail@robbertkrebbers.nl>
Date:   Wed Apr 17 14:54:44 2019 +0200

    Work.

commit 0fedd453c2ce41862f0a2040294ad0d271e39e85
Author: Jonas Kastberg Hinrichsen <jkas@itu.dk>
Date:   Wed Apr 17 12:55:52 2019 +0200

    Bumped Robbert feedback, WIP send st triple

commit f5672f9a529699ca0610329d32c59ad33d3146de
Author: Jonas Kastberg Hinrichsen <jkas@itu.dk>
Date:   Tue Apr 16 14:43:52 2019 +0200

    WIP

commit ef354c3899e796ccb091e1275e8b44d12a3393fd
Author: Jonas Kastberg Hinrichsen <jkas@itu.dk>
Date:   Tue Apr 16 13:39:41 2019 +0200

    Lifted stype over OFEs. Fixed residuals in channel.v

commit 1a47979d7497adb8c14ac9b57caf5632383ef2c3
Author: Jonas Kastberg Hinrichsen <jkas@itu.dk>
Date:   Tue Apr 16 13:08:28 2019 +0200

    WIP

commit 605562ba86b9481ae367409c87492b61d199111f
Author: Jonas Kastberg Hinrichsen <jkas@itu.dk>
Date:   Tue Apr 16 13:05:03 2019 +0200

    Test

commit 77eb6feb071da540fbc424602628c045ea15c004
Author: Robbert Krebbers <mail@robbertkrebbers.nl>
Date:   Mon Apr 15 16:24:13 2019 +0200

    Working.

theories/auth_excl.v
@@ -4,52 +4,64 @@ From iris.algebra Require Import excl auth.
 From iris.base_logic.lib Require Import auth.
 Set Default Proof Using "Type".
 
-Definition exclUR (A : Type) : ucmraT :=
-  optionUR (exclR (leibnizC A)).
+Class auth_exclG (A : ofeT) (Σ : gFunctors) := AuthExclG {
+  exclG_authG :> inG Σ (authR (optionUR (exclR A)));
+}.
 
-Class auth_exclG (A : Type) (Σ :gFunctors) :=
-  AuthExclG {
-      exclG_authG :> authG Σ (exclUR A);
-    }.
+Definition auth_exclΣ (F : cFunctor) `{!cFunctorContractive F} : gFunctors :=
+  #[GFunctor (authRF (optionURF (exclRF F)))].
 
-Definition auth_exclΣ (A : Type) : gFunctors :=
-  #[GFunctor (authR (exclUR A))].
-
-Instance subG_auth_exclG (A : Type) {Σ} :
-  subG (auth_exclΣ A) Σ → (auth_exclG A) Σ.
+Instance subG_auth_exclG (F : cFunctor) `{!cFunctorContractive F} {Σ} :
+  subG (auth_exclΣ F) Σ → auth_exclG (F (iPreProp Σ)) Σ.
 Proof. solve_inG. Qed.
 
-Definition to_auth_excl {A : Type} (a : A) : exclUR A :=
-  Excl' (a: leibnizC A).
+Definition to_auth_excl {A : ofeT} (a : A) : option (excl A) :=
+  Excl' a.
+Instance: Params (@to_auth_excl) 1.
+
+Section auth_excl_ofe.
+  Context {A : ofeT}.
+
+  Global Instance to_auth_excl_ne : NonExpansive (@to_auth_excl A).
+  Proof. solve_proper. Qed.
+
+  Global Instance to_auth_excl_proper :
+    Proper ((≡) ==> (≡)) (@to_auth_excl A).
+  Proof. solve_proper. Qed.
+End auth_excl_ofe.
 
 Section auth_excl.
   Context `{!auth_exclG A Σ}.
+  Implicit Types x y : A.
+
+  Lemma to_auth_excl_valid x y :
+    ✓ (● to_auth_excl x ⋅ ◯ to_auth_excl y) -∗ (x ≡ y : iProp Σ).
+  Proof.
+    iIntros "Hvalid".
+    iDestruct (auth_validI with "Hvalid") as "[Hy Hvalid]"; simpl.
+    iDestruct "Hy" as ([z|]) "Hy"; last first.
+    - by rewrite left_id right_id_L bi.option_equivI /= excl_equivI.
+    - iRewrite "Hy" in "Hvalid".
+      by rewrite left_id uPred.option_validI /= excl_validI /=.
+  Qed.
 
   Lemma excl_eq γ x y :
-    own γ (● to_auth_excl y) -∗ own γ (◯  to_auth_excl x) -∗ ⌜x = y⌝%I.
+    own γ (● to_auth_excl x) -∗ own γ (◯ to_auth_excl y) -∗ x ≡ y.
   Proof.
     iIntros "Hauth Hfrag".
-    iDestruct (own_valid_2 with "Hauth Hfrag") as %Hvalid.
-    apply auth_valid_discrete_2 in Hvalid.
-    destruct Hvalid as [Hincl _].
-    apply Excl_included in Hincl.
-    unfold to_auth_excl.
-    rewrite Hincl.
-    iFrame.
-    eauto.
+    iDestruct (own_valid_2 with "Hauth Hfrag") as "Hvalid".
+    iDestruct (to_auth_excl_valid with "Hvalid") as "$".
   Qed.
 
   Lemma excl_update γ x y z :
-    own γ (● to_auth_excl y) -∗ own γ (◯  to_auth_excl x) ==∗
-    own γ (● to_auth_excl z) ∗ own γ (◯  to_auth_excl z).
+    own γ (● to_auth_excl y) -∗ own γ (◯ to_auth_excl x) ==∗
+    own γ (● to_auth_excl z) ∗ own γ (◯ to_auth_excl z).
   Proof.
     iIntros "Hauth Hfrag".
     iDestruct (own_update_2 with "Hauth Hfrag") as "H".
     { eapply (auth_update _ _ (to_auth_excl z) (to_auth_excl z)).
       eapply option_local_update.
       eapply exclusive_local_update. done. }
-    rewrite own_op.
-    done.
+    by rewrite own_op.
   Qed.
-
 End auth_excl.
