theories/typing.v
@@ -1,41 +1,217 @@
 From iris.heap_lang Require Export lang.
-Require Import FunctionalExtensionality.
+From iris.algebra Require Export cmra.
+From stdpp Require Export list.
+From iris.base_logic Require Import base_logic.
+From iris.algebra Require Import updates local_updates.
+From iris.heap_lang Require Import proofmode notation.
+Set Default Proof Using "Type".
 
+Class Involutive {A} (R : relation A) (f : A → A) :=
+  involutive x : R (f (f x)) x.
 
-Class Involutive {T} (f : T → T) :=
-  involutive : ∀ t : T, t = f (f t).
-
-Inductive side : Set :=
-| Left
-| Right.
-
+Inductive side := Left | Right.
 Instance side_inhabited : Inhabited side := populate Left.
-
 Definition dual_side (s : side) : side :=
   match s with Left => Right | Right => Left end.
+Instance dual_side_involutive : Involutive (=) dual_side.
+Proof. by intros []. Qed.
 
-Instance dual_side_involutive : Involutive dual_side.
-Proof. intros s; destruct s; eauto. Qed.
+Inductive action := Send | Receive.
+Instance action_inhabited : Inhabited action := populate Send.
+Definition dual_action (a : action) : action :=
+  match a with Send => Receive | Receive => Send end.
+Instance dual_action_involutive : Involutive (=) dual_action.
+Proof. by intros []. Qed.
 
-Inductive stype :=
-| TEnd
-| TSend (P : val → Prop) (st : val → stype)
-| TRecv (P : val → Prop) (st : val → stype).
+Inductive stype (A : Type) :=
+  | TEnd
+  | TSR (a : action) (P : val → A) (st : val → stype A).
+Arguments TEnd {_}.
+Arguments TSR {_} _ _ _.
+Instance: Params (@TSR) 2.
 
-Instance stype_inhabited : Inhabited stype := populate TEnd.
+Instance stype_inhabited A : Inhabited (stype A) := populate TEnd.
 
-Fixpoint dual_stype (st :stype) :=
+Fixpoint dual_stype {A} (st : stype A) :=
   match st with
   | TEnd => TEnd
-  | TSend P st => TRecv P (λ v, dual_stype (st v))
-  | TRecv P st => TSend P (λ v, dual_stype (st v))
+  | TSR a P st => TSR (dual_action a) P (λ v, dual_stype (st v))
   end.
+Instance: Params (@dual_stype) 1.
 
-Instance dual_stype_involutive : Involutive dual_stype.
+Section stype_ofe.
+  Context {A : ofeT}.
+
+  Inductive stype_equiv : Equiv (stype A) :=
+    | TEnd_equiv : TEnd ≡ TEnd
+    | TSR_equiv a P1 P2 st1 st2 :
+       pointwise_relation val (≡) P1 P2 →
+       pointwise_relation val (≡) st1 st2 →
+       TSR a P1 st1 ≡ TSR a P2 st2.
+  Existing Instance stype_equiv.
+
+  Inductive stype_dist' (n : nat) : relation (stype A) :=
+    | TEnd_dist : stype_dist' n TEnd TEnd
+    | TSR_dist a P1 P2 st1 st2 :
+       pointwise_relation val (dist n) P1 P2 →
+       pointwise_relation val (stype_dist' n) st1 st2 →
+       stype_dist' n (TSR a P1 st1) (TSR a P2 st2).
+  Instance stype_dist : Dist (stype A) := stype_dist'.
+
+  Definition stype_ofe_mixin : OfeMixin (stype A).
+  Proof.
+    split.
+    - intros st1 st2. rewrite /dist /stype_dist. split.
+      + intros Hst n. induction Hst as [|a P1 P2 st1 st2 HP Hst IH]; constructor.
+        * intros v. apply equiv_dist, HP.
+        * intros v. apply IH.
+      + revert st2. induction st1 as [|a P1 st1 IH]; intros [|a' P2 st2] Hst.
+        * constructor.
+        * feed inversion (Hst O).
+        * feed inversion (Hst O).
+        * feed inversion (Hst O); subst.
+          constructor.
+          ** intros v. apply equiv_dist=> n. feed inversion (Hst n); subst; auto.
+          ** intros v. apply IH=> n. feed inversion (Hst n); subst; auto.
+    - rewrite /dist /stype_dist. split.
+      + intros st. induction st; constructor; repeat intro; auto.
+      + intros st1 st2. induction 1; constructor; repeat intro; auto.
+        symmetry; auto.
+      + intros st1 st2 st3 H1 H2.
+        revert H2. revert st3.
+        induction H1 as [| a P1 P2 st1 st2 HP Hst12 IH]=> //.
+        inversion 1. subst. constructor.
+        ** by transitivity P2.
+        ** intros v. by apply IH. 
+    - intros n st1 st2. induction 1; constructor.
+      + intros v. apply dist_S. apply H.
+      + intros v. apply H1.
+  Qed.
+  Canonical Structure stypeC : ofeT := OfeT (stype A) stype_ofe_mixin.
+
+  Global Instance TSR_stype_ne a n :
+    Proper (pointwise_relation _ (dist n) ==> pointwise_relation _ (dist n) ==> dist n) (TSR a).
+  Proof. 
+    intros P1 P2 HP st1 st2 Hst.
+    constructor.
+    - apply HP.
+    - intros v. apply Hst.
+  Qed.
+  Global Instance TSR_stype_proper a :
+    Proper (pointwise_relation _ (≡) ==> pointwise_relation _ (≡) ==> (≡)) (TSR a).
+  Proof.
+    intros P1 P2 HP st1 st2 Hst. apply equiv_dist=> n.
+    by f_equiv; intros v; apply equiv_dist.
+  Qed.
+
+  Global Instance dual_stype_ne : NonExpansive dual_stype.
+  Proof.
+    intros n. induction 1 as [| a P1 P2 st1 st2 HP Hst IH].
+    - constructor.
+    - constructor. apply HP. intros v. apply IH.
+  Qed.
+  Global Instance dual_stype_proper : Proper ((≡) ==> (≡)) dual_stype.
+  Proof. apply (ne_proper _). Qed.
+
+  Global Instance dual_stype_involutive : Involutive (≡) dual_stype.
+  Proof.
+    intros st.
+    induction st.
+    - constructor.
+    - rewrite /= (involutive (f:=dual_action)).
+      constructor. reflexivity. intros v. apply H.
+  Qed.
+  
+  Lemma stype_equivI {M} st1 st2 :
+    st1 ≡ st2 ⊣⊢@{uPredI M}
+        match st1, st2 with
+        | TEnd, TEnd => True
+        | TSR a1 P1 st1, TSR a2 P2 st2 =>
+          ⌜ a1 = a2 ⌝ ∧ (∀ v, P1 v ≡ P2 v) ∧ (∀ v, st1 v ≡ st2 v)
+        | _, _ => False
+        end.
+  Proof.
+    uPred.unseal; constructor=> n x ?. split; first by destruct 1.
+    destruct st1, st2=> //=; [constructor|].
+    by intros [[= ->] [??]]; constructor.
+  Qed.
+
+  Lemma dual_stype_flip {M} st1 st2 :
+    dual_stype st1 ≡ st2 ⊣⊢@{uPredI M} st1 ≡ dual_stype st2.
+  Proof.
+    iSplit.
+    - iIntros "Heq". iRewrite -"Heq". by rewrite dual_stype_involutive.
+    - iIntros "Heq". iRewrite "Heq". by rewrite dual_stype_involutive.
+  Qed.
+
+End stype_ofe.
+Arguments stypeC : clear implicits.
+
+Fixpoint stype_map {A B} (f : A → B) (st : stype A) : stype B :=
+  match st with
+  | TEnd => TEnd
+  | TSR a P st => TSR a (λ v, f (P v)) (λ v, stype_map f (st v))
+  end.
+Lemma stype_map_ext_ne {A} {B : ofeT} (f g : A → B) (st : stype A) n :
+  (∀ x, f x ≡{n}≡ g x) → stype_map f st ≡{n}≡ stype_map g st.
 Proof.
-  intros st.
-  induction st => //; simpl;
-    assert (st = (λ v : val, dual_stype (dual_stype (st v)))) as Heq
-        by apply functional_extensionality => //;
-    rewrite -Heq => //.
+  intros Hf. induction st as [| a P st IH]; constructor.
+  - intros v. apply Hf.
+  - intros v. apply IH.
 Qed.
+Lemma stype_map_ext {A} {B : ofeT} (f g : A → B) (st : stype A) :
+  (∀ x, f x ≡ g x) → stype_map f st ≡ stype_map g st.
+Proof.
+  intros Hf. apply equiv_dist.
+  intros n. apply stype_map_ext_ne.
+  intros x. apply equiv_dist.
+  apply Hf.
+Qed.
+Instance stype_map_ne {A B : ofeT} (f : A → B) n:
+  Proper (dist n ==> dist n) f → Proper (dist n ==> dist n) (stype_map f).
+Proof.
+  intros Hf st1 st2. induction 1 as [| a P1 P2 st1 st2 HP Hst IH]; constructor.
+  - intros v. f_equiv. apply HP.
+  - intros v. apply IH.
+Qed.
+Lemma stype_fmap_id {A : ofeT} (st : stype A) : stype_map id st ≡ st.
+Proof.
+  induction st as [| a P st IH]; constructor.
+  - intros v. reflexivity.
+  - intros v. apply IH.
+Qed.
+Lemma stype_fmap_compose {A B C : ofeT} (f : A → B) (g : B → C) st :
+  stype_map (g ∘ f) st ≡ stype_map g (stype_map f st).
+Proof.
+  induction st as [| a P st IH]; constructor.
+  - intros v. reflexivity.
+  - intros v. apply IH.
+Qed.
+
+Definition stypeC_map {A B} (f : A -n> B) : stypeC A -n> stypeC B :=
+  CofeMor (stype_map f : stypeC A → stypeC B).
+Instance stypeC_map_ne A B : NonExpansive (@stypeC_map A B).
+Proof. intros n f g ? st. by apply stype_map_ext_ne. Qed.
+
+Program Definition stypeCF (F : cFunctor) : cFunctor := {|
+  cFunctor_car A B := stypeC (cFunctor_car F A B);
+  cFunctor_map A1 A2 B1 B2 fg := stypeC_map (cFunctor_map F fg)
+|}.
+Next Obligation.
+  by intros F A1 A2 B1 B2 n f g Hfg; apply stypeC_map_ne, cFunctor_ne.
+Qed.
+Next Obligation.
+  intros F A B x. rewrite /= -{2}(stype_fmap_id x).
+  apply stype_map_ext=>y. apply cFunctor_id.
+Qed.
+Next Obligation.
+  intros F A1 A2 A3 B1 B2 B3 f g f' g' x. rewrite /= -stype_fmap_compose.
+  apply stype_map_ext=>y; apply cFunctor_compose.
+Qed.
+
+Instance stypeCF_contractive F :
+  cFunctorContractive F → cFunctorContractive (stypeCF F).
+Proof.
+  by intros ? A1 A2 B1 B2 n f g Hfg; apply stypeC_map_ne, cFunctor_contractive.
+Qed.
+
